Improve def of fresh

src/fresh.lean
@@ -6,24 +6,25 @@ variables {L L₁ L₂ : finset V} -- Variable sets
 variables {x : V} -- Variables
 variables {xs : list V} -- Lists of variables
 
-def fresh : list V → finset V → Prop
-  | []        L := true
-  | (x :: xs) L := x ∉ L ∧ fresh xs (insert x L)
+-- Freshness of a list of variables from a set L and from one another
+def fresh (L : finset V) : list V → Prop
+  | []        := true
+  | (x :: xs) := x ∉ xs ∧ x ∉ L ∧ fresh xs
 
 @[simp]
-theorem fresh_nil : fresh [] L ↔ true :=
+theorem fresh_nil : fresh L [] ↔ true :=
   by rw fresh
 
 @[simp]
-theorem fresh_cons : fresh (x :: xs) L ↔ x ∉ L ∧ fresh xs (insert x L) :=
+theorem fresh_cons : fresh L (x :: xs) ↔ x ∉ xs ∧ x ∉ L ∧ fresh L xs :=
   by rw fresh
 
 @[simp]
-theorem fresh_union : fresh xs (L₁ ∪ L₂) ↔ fresh xs L₁ ∧ fresh xs L₂ :=
+theorem fresh_union : fresh (L₁ ∪ L₂) xs ↔ fresh L₁ xs ∧ fresh L₂ xs :=
   begin
-    induction xs with hd tl ih generalizing L₁ L₂; simp [decidable.not_or_iff_and_not, and.assoc],
-    rw [finset.insert_union_distrib hd L₁ L₂, ih],
-    simp [and.left_comm]
+    induction xs with hd tl ih generalizing L₁ L₂; simp [decidable.not_or_iff_and_not, and.assoc, and.left_comm],
+    rw ih,
+    exact ⟨λ ⟨a, b, c, d, e⟩, ⟨a, b, c, c, d, e⟩, λ ⟨a, b, c, _, d, e⟩, ⟨a, b, c, d, e⟩⟩
   end
 
 end /- namespace -/ tts --------------------------------------------------------
