src/sch/defs.lean
@@ -40,7 +40,7 @@ variables [_root_.decidable_eq V]
 
 -- Property of a scheme body.
 def body (n : ℕ) (t : typ V) : Prop :=
-  ∃ (L : finset V), ∀ (xs : list V), n = xs.length → fresh xs L → (t.open_vars xs).lc
+  ∃ (L : finset V), ∀ (xs : list V), n = xs.length → fresh L xs → (t.open_vars xs).lc
 
 -- Property of a well-formed scheme.
 def well_formed (s : sch V) : Prop :=
